Prove more cases, but approach is still doomed
Magnus suggested insisting that the code tables be empty, and this does
make the Call case go through, and this will certainly make the eventual
proof easier, but the value relation is still wrong (evaluate_app
reveals the problem). I'm back to being convinced that the various
relations need to be parameterised by the env-approximation and globals
approximation information (à la what things looked like in de4c64918b5).

compiler/backend/proofs/clos_knownProofScript.sml
@@ -1465,7 +1465,7 @@ val ksrel_def = Define`
      s2.clock = s1.clock ∧ s2.ffi = s1.ffi ∧
      LIST_REL (OPTREL kvrel) s1.globals s2.globals ∧
      fmap_rel (ref_rel kvrel) s1.refs s2.refs ∧
-     fmap_rel (λ(n1,e1) (n2,e2). n1 = n2 ∧ kerel e1 e2) s1.code s2.code
+     s1.code = FEMPTY ∧ s2.code = FEMPTY
 `;
 
 (* ksrel necessary *)
@@ -1487,13 +1487,6 @@ val ksrel_ssgc_free = Q.store_thm(
   `ksrel s1 s2 ⇒ (ssgc_free s1 ⇔ ssgc_free s2)`,
   simp[ksrel_def, ssgc_free_def] >> rpt strip_tac >> eq_tac >> rpt strip_tac >>
   fs[fmap_rel_OPTREL_FLOOKUP]
-  >- (qcase_tac `FLOOKUP s2.code kk = SOME (mm,ee)` >>
-      `OPTREL (λ(n1,e1) (n2,e2). n1 = n2 ∧ kerel e1 e2)
-              (FLOOKUP s1.code kk) (FLOOKUP s2.code kk)`
-        by metis_tac[] >> pop_assum mp_tac >>
-      simp_tac (srw_ss()) [OPTREL_def] >> simp[EXISTS_PROD] >>
-      rpt strip_tac >> res_tac >> fs[kerel_def] >> rw[] >>
-      imp_res_tac known_preserves_setGlobals >> fs[])
   >- (qcase_tac `FLOOKUP s2.refs kk = SOME (ValueArray vvl)` >>
       `OPTREL (ref_rel kvrel) (FLOOKUP s1.refs kk) (FLOOKUP s2.refs kk)`
          by simp[] >> pop_assum mp_tac >>
@@ -1505,13 +1498,6 @@ val ksrel_ssgc_free = Q.store_thm(
       `OPTREL kvrel (EL kk s1.globals) (EL kk s2.globals)` by simp[] >>
       pop_assum mp_tac >> simp_tac(srw_ss()) [OPTREL_def] >> simp[] >>
       metis_tac[kvrel_vsgc_free, MEM_EL])
-  >- (qcase_tac `FLOOKUP s1.code kk = SOME (mm,ee)` >>
-      `OPTREL (λ(n1,e1) (n2,e2). n1 = n2 ∧ kerel e1 e2)
-              (FLOOKUP s1.code kk) (FLOOKUP s2.code kk)`
-        by metis_tac[] >> pop_assum mp_tac >>
-      simp_tac (srw_ss()) [OPTREL_def] >> simp[EXISTS_PROD] >>
-      rpt strip_tac >> res_tac >> fs[kerel_def] >> rw[] >>
-      imp_res_tac known_preserves_setGlobals >> fs[])
   >- (qcase_tac `FLOOKUP s1.refs kk = SOME (ValueArray vvl)` >>
       `OPTREL (ref_rel kvrel) (FLOOKUP s1.refs kk) (FLOOKUP s2.refs kk)`
          by simp[] >> pop_assum mp_tac >>
@@ -1690,33 +1676,77 @@ val loptrel_def = Define`
      lopt2 = lopt1 ∨
      lopt1 = NONE ∧
      case (fv,lopt2) of
-       | (Closure (SOME loc1) _ _ n bod, SOME loc2) => loc1 = loc2 ∧ n = numargs
-       | (Recclosure (SOME loc1) _ _ fns i, SOME loc2) =>
-         i < LENGTH fns ∧ loc2 = loc1 + i ∧ numargs = FST (EL i fns)
-       | _ => T
+       | (Closure (SOME loc1) ae _ n bod, SOME loc2) =>
+            loc1 = loc2 ∧ n = numargs ∧ ae = []
+       | (Recclosure (SOME loc1) ae _ fns i, SOME loc2) =>
+         i < LENGTH fns ∧ loc2 = loc1 + i ∧ numargs = FST (EL i fns) ∧
+         ae = []
+       | _ => F
 `;
 
-val ksrel_find_code_SOME = Q.store_thm(
-  "ksrel_find_code_SOME",
-  `ksrel s1 s2 ∧ LIST_REL kvrel vs1 vs2 ∧
-   find_code l vs1 s1.code = SOME (args1,e1) ⇒
-   ∃args2 e2. find_code l vs2 s2.code = SOME(args2,e2) ∧
-              LIST_REL kvrel args1 args2 ∧
-              kerel e1 e2`,
-  simp[ksrel_def, find_code_def, eqs, pair_case_eq] >>
-  simp[fmap_rel_OPTREL_FLOOKUP] >> rpt strip_tac >>
-  rpt (first_x_assum (qspec_then `l` mp_tac)) >>
-  simp[OPTREL_def, EXISTS_PROD] >> fs[LIST_REL_EL_EQN]);
+val ksrel_find_code = Q.store_thm(
+  "ksrel_find_code",
+  `ksrel s1 s2 ⇒ find_code l (vs1:closSem$v list) s1.code = NONE`,
+  simp[ksrel_def, find_code_def, eqs, pair_case_eq]);
 
-val ksrel_find_code_NONE = Q.store_thm(
-  "ksrel_find_code_NONE",
-  `ksrel s1 s2 ∧ LIST_REL kvrel vs1 vs2 ∧ find_code l vs1 s1.code = NONE ⇒
-   find_code l vs2 s2.code = NONE`,
-  simp[ksrel_def, find_code_def, eqs, pair_case_eq, fmap_rel_OPTREL_FLOOKUP] >>
-  rpt strip_tac >>
-  rpt (first_x_assum (qspec_then `l` mp_tac)) >>
-  simp[OPTREL_def, EXISTS_PROD] >> fs[LIST_REL_EL_EQN] >> rpt strip_tac >>
-  simp[]);
+val kvrel_dest_closure_SOME_Partial = Q.store_thm(
+  "kvrel_dest_closure_SOME_Partial",
+  `dest_closure lopt1 f1 vs1 = SOME (Partial_app v1) ∧ kvrel f1 f2 ∧
+   LIST_REL kvrel vs1 vs2 ∧ loptrel f2 n lopt1 lopt2 ∧ LENGTH vs2 = n ⇒
+   ∃v2. dest_closure lopt2 f2 vs2 = SOME (Partial_app v2) ∧
+        kvrel v1 v2`,
+  simp[dest_closure_def, eqs, v_case_eq] >> rpt strip_tac >> rveq >> fs[] >>
+  rpt strip_tac >> fs[eqs, bool_case_eq] >> rveq >> fs[loptrel_def] >> rveq
+  >- (reverse (rpt strip_tac) >- simp[EVERY2_APPEND_suff] >>
+      fs[LIST_REL_EL_EQN])
+  >- (Cases_on `lopt2` >> simp[EVERY2_APPEND_suff] >> fs[LIST_REL_EL_EQN] >>
+      qcase_tac `option_CASE lll` >> Cases_on `lll` >> fs[LIST_REL_EL_EQN])
+  >- (rpt (pairarg_tac >> fs[]) >> fs[bool_case_eq] >>
+      simp[EVERY2_APPEND_suff] >>
+      fs[LIST_REL_EL_EQN] >> qcase_tac `EL ii` >>
+      qpat_assum `∀n. _ ⇒ UNCURRY f x y` mp_tac >>
+      disch_then (qspec_then `ii` mp_tac) >> simp[] >> rw[] >>
+      fs[LIST_REL_EL_EQN])
+  >- (rpt (pairarg_tac >> fs[]) >> fs[bool_case_eq] >>
+      Cases_on `lopt2` >> fs[] >> qcase_tac `option_CASE lll` >>
+      Cases_on `lll` >> fs[] >> rveq >>
+      qpat_assum `LIST_REL (UNCURRY _) _ _` mp_tac >>
+      CONV_TAC (LAND_CONV (REWRITE_CONV [LIST_REL_EL_EQN])) >>
+      qcase_tac `EL ii` >>
+      disch_then (CONJUNCTS_THEN2 assume_tac (qspec_then `ii` mp_tac)) >>
+      strip_tac >> rfs[] >> fs[LIST_REL_EL_EQN]))
+
+val kvrel_dest_closure_SOME_Full = Q.store_thm(
+  "kvrel_dest_closure_SOME_Full",
+  `dest_closure lopt1 f1 vs1 = SOME (Full_app e1 env1 args1) ∧ kvrel f1 f2 ∧
+   LIST_REL kvrel vs1 vs2 ∧ loptrel f2 n lopt1 lopt2 ∧ LENGTH vs2 = n ⇒
+   ∃e2 env2 args2.
+      dest_closure lopt2 f2 vs2 = SOME (Full_app e2 env2 args2) ∧
+      LIST_REL kvrel env1 env2 ∧ LIST_REL kvrel args1 args2 ∧
+      kerel e1 e2`,
+  simp[dest_closure_def, eqs, bool_case_eq] >>
+  csimp[revtakerev, revdroprev] >> dsimp[] >> rpt strip_tac >> rveq >>
+  fs[] >> rveq >> fs[]
+  >- (imp_res_tac LIST_REL_LENGTH >> simp[] >> fs[] >>
+      simp[EVERY2_APPEND_suff, EVERY2_DROP, EVERY2_TAKE] >>
+      fs[loptrel_def] >> Cases_on `lopt2` >> fs[] >>
+      qcase_tac `option_CASE lll` >> Cases_on `lll` >> fs[] >> rveq >>
+      fs[check_loc_def])
+  >- (rpt (pairarg_tac >> fs[]) >> imp_res_tac LIST_REL_LENGTH >> fs[] >>
+      fs[bool_case_eq] >> rveq >>
+      qpat_assum `LIST_REL (UNCURRY _) _ _`
+        (fn th => (mp_tac o SIMP_RULE (srw_ss()) [LIST_REL_EL_EQN]) th >>
+                  assume_tac th) >>
+      qcase_tac `EL ii` >> simp[] >>
+      disch_then (qspec_then `ii` mp_tac) >> simp[] >> strip_tac >> rveq >>
+      reverse conj_tac
+      >- (simp[EVERY2_TAKE] >>
+          rpt (irule EVERY2_APPEND_suff) >> simp[EVERY2_DROP, EVERY2_TAKE] >>
+          simp[LIST_REL_GENLIST]) >>
+      fs[loptrel_def] >> Cases_on `lopt2` >> fs[] >>
+      qcase_tac `option_CASE lll` >> Cases_on `lll` >> fs[] >>
+      fs[check_loc_def]))
+
 
 val known_correct0 = Q.prove(
   `(∀a es env1 env2 (s01:α closSem$state) s02 res1 s1 g0 g as ealist.
@@ -2032,24 +2062,59 @@ val known_correct0 = Q.prove(
       >- (simp[] >> metis_tac[pair_CASES])
       >- (rpt (pairarg_tac >> fs[]) >> rveq >> nailIHx strip_assume_tac >>
           simp[evaluate_def] >> rw[] >>
-          map_every qcase_tac [
-            `evaluate(MAP FST alist,env2,s02) = (Rval vs2,s2)`,
-            `ksrel s01 s02`,
-            `evaluate (exps1,env1,s01) = (Rval vs1, s1)`,
-            `known exps1 apxs g0 = (alist,g)`,
-            `ksrel s1 s2`] >>
-          `∃args2 e2. find_code dest vs2 s2.code = SOME(args2,e2)`
-             by metis_tac[ksrel_find_code_SOME] >> dsimp[bool_case_eq] >>
-          `s2.clock = 0` by fs[ksrel_def] >> simp[])
+          imp_res_tac ksrel_find_code >> fs[])
       >- (fixeqs >> rpt (pairarg_tac >> fs[]) >> rveq >> fs[] >>
-          nailIHx strip_assume_tac >> simp[evaluate_def] >> cheat)
+          nailIHx strip_assume_tac >>
+          imp_res_tac ksrel_find_code >> fs[])
       >- (rpt (pairarg_tac >> fs[]) >> rveq >> fs[] >>
           nailIHx strip_assume_tac >> simp[evaluate_def] >>
           fs[krrel_err_rw] >>
           dsimp[result_case_eq, eqs, pair_case_eq, bool_case_eq] >>
           metis_tac[option_CASES, pair_CASES, result_CASES]))
-  >- (say "evaluate_app(nil)" >> cheat)
-  >- (say "evaluate_app(cons)" >> cheat))
+  >- (say "evaluate_app(nil)" >> simp[evaluate_def])
+  >- (say "evaluate_app(cons)" >> rpt gen_tac >> strip_tac >>
+      simp[evaluate_def, eqs, bool_case_eq, pair_case_eq, result_case_eq] >>
+      rpt strip_tac >> rveq >> fs[]
+      >- metis_tac[pair_CASES]
+      >- (simp[evaluate_def, eqs, bool_case_eq] >>
+          first_assum
+            (mp_tac o
+             asmPART_MATCH' hd (GEN_ALL kvrel_dest_closure_SOME_Partial) o
+             concl) >> simp[PULL_EXISTS] >> strip_tac >>
+          sel_ihpc hd >> simp[] >> strip_tac >> sel_ihpc hd >> simp[] >>
+          strip_tac >> sel_ihpc hd >> imp_res_tac LIST_REL_LENGTH >>
+          strip_tac >> fs[] >> nailIHx strip_assume_tac >> simp[] >>
+          fs[ksrel_def])
+      >- (simp[evaluate_def, eqs, bool_case_eq] >>
+          first_assum
+            (mp_tac o
+             asmPART_MATCH' hd (GEN_ALL kvrel_dest_closure_SOME_Partial) o
+             concl) >> simp[PULL_EXISTS] >> strip_tac >>
+          sel_ihpc (el 3) >> simp[] >> imp_res_tac LIST_REL_LENGTH >> fs[] >>
+          strip_tac >> nailIHx strip_assume_tac >> simp[] >>
+          fs[ksrel_def, dec_clock_def])
+      >- (simp[evaluate_def, eqs, bool_case_eq] >>
+          first_assum
+            (mp_tac o
+             asmPART_MATCH' hd (GEN_ALL kvrel_dest_closure_SOME_Full) o
+             concl) >> simp[PULL_EXISTS] >> strip_tac >>
+          sel_ihpc (el 3) >> simp[] >> imp_res_tac LIST_REL_LENGTH >> fs[] >>
+          strip_tac >> nailIHx strip_assume_tac >> simp[] >>
+          `s02.clock = s01.clock` by fs[ksrel_def] >>
+          imp_res_tac LIST_REL_LENGTH >> fs[] >>
+          fs[ksrel_def])
+      >- (simp[evaluate_def, eqs, bool_case_eq, pair_case_eq] >>
+          first_assum
+            (mp_tac o
+             asmPART_MATCH' hd (GEN_ALL kvrel_dest_closure_SOME_Full) o
+             concl) >> simp[PULL_EXISTS] >> strip_tac >>
+          sel_ihpc (el 3) >> simp[] >> imp_res_tac LIST_REL_LENGTH >> fs[] >>
+          strip_tac >> nailIHx strip_assume_tac >> simp[] >>
+          `s02.clock = s01.clock` by fs[ksrel_def] >>
+          imp_res_tac LIST_REL_LENGTH >> fs[] >> simp[PULL_EXISTS] >>
+          dsimp[] >> fs[PULL_EXISTS] >> cheat)
+      >- (imp_res_tac evaluate_SING >> fs[])
+      >- cheat))
 
 val known_correct = save_thm(
   "known_correct",
